vvequiv/NetlistSemantics.v
@@ -25,18 +25,20 @@ Equations input_port_in_map : NameMap.t bv -> (name * port_direction) -> Prop :=
 Record ExternalState (c : circuit) :=
   MkExternalState
     { external_state_map :> NameMap.t bv
-    ; external_state_match_circuit : Forall (input_port_in_map external_state_map) (circuitPorts c)
+    ; external_state_match_circuit :
+      forall n, NameMap.In n (circuitPorts c) -> NameMap.In n external_state_map
     }.
 
 Arguments MkExternalState [_] _ _.
 
-Equations register_in_map : NameMap.t bv -> register_declaration -> Prop :=
-| map, MkRegister (Logic w) n _ _ => exists bv, NameMap.MapsTo n bv map /\ width bv = w.
-
 Record RegisterState (c : circuit) :=
   MkRegisterState
     { register_state_map :> NameMap.t bv
-    ; register_state_wf : Forall (register_in_map register_state_map) (circuitRegisters c)
+    ; register_state_wf :
+      forall n t i d,
+        NameMap.MapsTo n (MkRegister t i d) (circuitRegisters c)
+        -> (exists v, NameMap.MapsTo n v register_state_map /\ (width v = type_width t))
+
     }.
 
 Arguments MkRegisterState [_] _ _.
@@ -47,7 +49,10 @@ Equations variable_in_map : NameMap.t bv -> variable -> Prop :=
 Record VariableState (c : circuit) :=
   MkVariableState
     { variable_state_map :> NameMap.t bv
-    ; variable_state_wf : Forall (variable_in_map variable_state_map) (circuitVariables c)
+    ; variable_state_wf :
+      forall n t,
+        NameMap.MapsTo n t (circuitVariables c)
+        -> (exists v, NameMap.MapsTo n v variable_state_map /\ (width v = type_width t))
     }.
 
 Arguments MkVariableState [_] _ _.
@@ -70,16 +75,14 @@ Set Primitive Projections.
 Equations varWidth : variable -> positive :=
   varWidth (Var (Logic w) _) := w.
 
-Equations var_reg_match : variable -> register_declaration -> Prop :=
-| Var var_type var_name, MkRegister reg_type reg_name _ _ =>
-    var_type = reg_type /\ var_name = reg_name.
-
 Equations input_in_circuit : circuit -> input -> Prop :=
 | _, InConstant _ => True
-| c, InVar v => In v (circuitVariables c) \/ Exists (var_reg_match v) (circuitRegisters c).
+| c, InVar (Var t n) => NameMap.MapsTo n t (circuitVariables c).
+
 
 Equations output_in_circuit : circuit -> output -> Prop :=
-| c, OutVar v => In v (circuitVariables c) \/ Exists (var_reg_match v) (circuitRegisters c).
+| c, OutVar (Var t n) => NameMap.MapsTo n t (circuitVariables c).
+
 
 Equations cell_in_circuit : circuit -> cell -> Prop :=
 | c, Add out in1 in2 _ _ =>
@@ -98,65 +101,44 @@ Equations cell_in_circuit : circuit -> cell -> Prop :=
     /\ input_in_circuit c in1
 .
 
-Set Equations With UIP.
 
 Equations input_run {c} (st : CircuitState c) (i : input) (input_wf : input_in_circuit c i) : bv :=
   input_run st (InConstant const) _ := const;
-  input_run st (InVar v) input_wf
-    with NameMap.find v.(varName) st.(registers), NameMap.find v.(varName) st.(variables) => {
-    | Some x, _ => x
-    | _, Some x => x
-    | None, None => _
-    }.
+  input_run st (InVar (Var t n)) wf with NameMap.find n (variables st) => {
+    | Some x := x;
+    | None with (_ : False) => { | ! }
+    }
+.
 Next Obligation.
+  (* Lookup always succeeds *)
 Admitted.
-(*   exfalso. *)
-(*   rewrite <- NameMapFacts.not_find_in_iff in *. *)
-(*   destruct input_wf. *)
-(*   - apply Evariables. clear Evariables. clear Eregisters. *)
-(*     destruct st as [exts regs vars]. simpl in *. *)
-(*     destruct vars as [var_map vars_wf]. *)
-(*     simpl. *)
-(*     rewrite Forall_forall in vars_wf. *)
-(*     apply vars_wf in H. clear vars_wf. *)
-(*     funelim (variable_in_map var_map v). *)
-(*     simp variable_in_map in H. *)
-(*     destruct H as [bv [Hmap _]]. *)
-(*     eexists. eauto. *)
-(*   - apply Eregisters. clear Evariables. clear Eregisters. *)
-(*     rewrite Exists_exists in H. *)
-(*     destruct H as [r [H1 H2]]. *)
-(*     destruct st as [exts regs vars]. simpl in *. *)
-(*     destruct regs as [reg_map regs_wf]. *)
-(*     simpl in *. *)
-(*     rewrite Forall_forall in regs_wf. *)
-(*     apply regs_wf in H1. *)
-(*     funelim (register_in_map reg_map r). *)
-(*     funelim (var_reg_match v (MkRegister (Logic w) n init driver)). *)
-(*     simp register_in_map in *. *)
-(*     simp var_reg_match in *. *)
-(*     simpl in *. *)
-(*     inversion H2; subst. *)
-(*     destruct H1 as [bv [Hmap _]]. *)
-(*     eexists. eassumption. *)
-(* Defined. *)
+
+
+(* Lemma input_width : forall c n t1 t2, input_in_circuit c (Var t1 n) -> NameMap.MapsTo n t2 (circuitVariables c) -> t1 = t2. *)
 
 Lemma input_run_width : forall {c} (st : CircuitState c) i input_wf,
     width (input_run st i input_wf) = input_width i.
 Proof.
   intros.
+  destruct st as [exts regs [vars vars_wf]].
   funelim (input_width i).
   - simp input_run.
+    unfold input_run_clause_2.
     simpl.
-    unfold input_run_clause_2_clause_1.
-    destruct (NameMap.find varName0 (registers st)) eqn:Ereg.
-    + admit.
-    + destruct (NameMap.find varName0 (variables st)) eqn:Evars.
-      * admit.
-      * inversion input_wf.
-        rewrite <- NameMapFacts.not_find_in_iff in Evars.
+    assert (exists b, NameMap.find varName0 vars = Some b) as [b Hb]. {
+      simp input_in_circuit in input_wf.
+      edestruct vars_wf as [b' [Hvars Hwidth]]; eauto.
+    }
+    destruct (NameMap.find varName0 vars) eqn:E. 2: solve [discriminate].
+    inversion Hb; subst; clear Hb.
+    simp input_in_circuit in input_wf.
+    edestruct vars_wf as [b' [Hvars Hwidth]]; eauto.
+    replace b with b'.
+    + simp type_width in *.
+    + rewrite <- NameMapFacts.find_mapsto_iff in E.
+      eauto using NameMapFacts.MapsTo_fun.
   - simp input_run. reflexivity.
-Admitted.
+Qed.
 
 Lemma variable_in_map_extend_other : forall (k : NameMap.key) (t : nltype) (n : name) (x: bv) (m : NameMap.t bv),
     n <> k -> variable_in_map m (Var t n) -> variable_in_map (NameMap.add k x m) (Var t n).
@@ -180,7 +162,7 @@ Proof.
   inversion H; subst; clear H.
   simp variable_in_map in *.
   destruct Hin as [xprev [Hmap Hwidth]].
-  destruct (Pos.eq_dec n0 k).
+  compare n0 k; intros E.
   - subst.
     exists x.
     intuition.
@@ -203,7 +185,30 @@ Proof.
   - auto using variable_in_map_extend_same.
 Qed.
 
-Ltac simpl_list_props := repeat (try rewrite Forall_forall in *; try rewrite Exists_exists in *).
+(* Ltac simpl_list_props := repeat (try rewrite Forall_forall in *; try rewrite Exists_exists in .*)
+
+Ltac inv_circuit_state st :=
+  destruct st as [[exts exts_wf] [regs regs_wf] [vars vars_wf]].
+
+Lemma circuit_to_state_variables : forall c (st: CircuitState c) n t,
+    NameMap.MapsTo n t (circuitVariables c) ->
+    exists v, (NameMap.MapsTo n v (variables st) /\ width v = type_width t).
+Proof.
+  intros * H.
+  inv_circuit_state st.
+  simpl in *.
+  edestruct vars_wf as [v [Hvars _]]; eauto.
+Qed.
+
+(* Lemma state_to_circuit_variables : forall c (st: CircuitState c) n v, *)
+(*     NameMap.MapsTo n v (variables st) -> *)
+(*     NameMap.MapsTo n (Logic (width v)) (circuitVariables c). *)
+(* Proof. *)
+(*   intros * H. *)
+(*   inv_circuit_state st. *)
+(*   destruct (vars_wf n (Logic (width v))) as [_ vars_wf_to]. *)
+(*   eauto. *)
+(* Qed. *)
 
 Equations cell_run {c} (st : CircuitState c) (cl : cell) (cell_wf : cell_in_circuit c cl) : CircuitState c :=
   cell_run st (Add (OutVar (Var _ out)) in1 in2 inputs_match output_match) cell_wf :=
@@ -231,21 +236,28 @@ Next Obligation.
   assumption.
 Qed.
 Next Obligation.
-  destruct st as [exts regs vars].
-  destruct vars as [vars_map vars_wf].
-  simpl in *.
-  pose proof vars_wf as vars_wf_forall.
-  simpl_list_props.
-  intros [[xwidth] xname] Hin.
-  destruct (Pos.eq_dec xname out).
-  - subst.
-    apply variable_in_map_extend_same.
-    + rewrite bv_add_truncate_width.
-      rewrite input_run_width.
-      admit. (* Need that circuitVariables is a map from names to types (equal names -> equal types) *)
-    + auto.
-  - auto using variable_in_map_extend_other.
-Admitted.
+  compare n out; intros E.
+  + subst. eexists.
+    NameMapFacts.map_iff.
+    intuition eauto.
+    rewrite bv_add_truncate_width.
+    rewrite input_run_width.
+    rewrite output_match.
+    inversion cell_wf as [Hout _]. clear cell_wf.
+    funelim (output_width _).
+    inversion eqargs; subst; clear eqargs.
+    clear inputs_match. clear output_match. clear in1. clear in2.
+    simp output_in_circuit in *.
+    destruct t as [w'].
+    assert (Logic w = Logic w') as Hw by eauto using NameMapFacts.MapsTo_fun.
+    inversion Hw; subst; clear Hw.
+    simp type_width.
+    trivial.
+  + edestruct circuit_to_state_variables as [v [Hv_in Hv_width]]; eauto.
+    exists v.
+    erewrite NameMapFacts.add_mapsto_iff.
+    intuition eauto.
+Qed.
 
 Equations circuit_run
   (fext : ExternalState)
